fold.v
@@ -1,0 +1,165 @@
+Require Import QArith.
+Require Import Qcanon.
+Require Import MyVector.
+Require Import List.
+Require Import ZArith.
+Add LoadPath "../../src/cslsound".
+Require Import Lang.
+
+Set Implicit Arguments.
+Unset Strict Implicit.
+
+Require Import PHeap.
+Require Import Bdiv.
+Require Import CSL.
+
+Close Scope Qc_scope.
+Close Scope Q_scope.
+
+Section Fold.
+  Notation tid := (0%Z : var).
+  Notation x := (1%Z : var).
+  Notation y := (2%Z : var).
+  Notation r := (3%Z : var).
+  Notation arr := (4%Z : var).
+
+  Variable n : Z.
+  Variable ntrd : nat.
+
+  Bind Scope exp_scope with exp.
+  Bind Scope bexp_scope with bexp.
+  
+  Infix "+" := (Eplus) : exp_scope.
+  Infix "<" := (Blt) : bexp_scope.
+  Infix "==" := (Beq) : bexp_scope.
+  Coercion Evar : var >-> exp.
+  Coercion Enum : Z >-> exp.
+  Open Scope exp_scope.
+  Open Scope bexp_scope.
+
+  Fixpoint is_array (e : exp) (n : nat) (f : nat -> Z) :=
+    match n with
+      | 0 => Aemp
+      | S n' => Adisj (Aex (fun v => Apointsto 1%Qc (e + Z.of_nat n) v))
+                      (is_array e n' f)
+    end.
+
+
+  Bind Scope assn_scope with assn.
+  Notation "P '//\\' Q" := (fun s h => P s h /\ Q s h) (at level 80, right associativity) : assn_scope.
+  Notation "x '===' y" := 
+    (fun s h => edenot x s = edenot y s) (at level 70, no associativity) 
+    : assn_scope.
+  Notation "'existS' x .. y , p" := 
+    (fun s h => ex (fun x => .. (ex (fun y => p s h)) ..))
+      (at level 200, x binder, y binder, right associativity) : assn_scope.
+  Notation "e1 '-->p' ( p ,  e2 )" := (Apointsto p e1 e2) (at level 75) : assn_scope.
+  Delimit Scope assn_scope with assn.
+
+  Variable f : nat -> Z.
+
+  Definition nat_of_fin (i : Fin.t ntrd) : nat := projT1 (Fin.to_nat i).
+  Definition Z_of_fin (i : Fin.t ntrd) : Z := Z.of_nat (nat_of_fin i).
+
+  Section Rotate.
+    Notation ntrdZ := (Z_of_nat ntrd).
+    Definition rotate := 
+      x ::= [arr + tid] ;;
+      Cbarrier 0 ;;
+      Cif (r == ntrdZ) (
+        y ::= 0%Z
+      ) (
+        y ::= tid + 1%Z
+      ) ;;
+      [arr + y] ::= x.
+    Definition Pre := is_array arr (ntrd + 1) (fun i => Z.of_nat i).
+    Definition Post := is_array arr (ntrd + 1) (fun i : nat => (Z.of_nat i - 1) mod ntrdZ)%Z.
+    Definition Pre_i := (arr + tid -->p (1%Qc, tid))%assn.
+    Definition Post_i := (arr + ((tid + 1) mod ntrdZ)%Z -->p (1%Qc, tid))%assn.
+    
+    Definition E (var : var) := 
+      if Z.eq_dec var tid then Hi
+      else if Z.eq_dec var x then Hi
+      else if Z.eq_dec var y then Hi
+      else Lo.
+
+    Definition bpre (tid : Fin.t ntrd) := 
+      (arr + (Z_of_fin tid) -->p (1%Qc, Z_of_fin tid))%assn.
+    Definition bpost (tid : Fin.t ntrd) := 
+      (arr + (((Z_of_fin tid) + 1) mod ntrdZ)%Z -->p (1%Qc, Z_of_fin tid))%assn.
+
+    Lemma pre_lassn (tid : Fin.t ntrd) : low_assn E (bpre tid).
+    Proof.
+      unfold low_assn, Bdiv.low_assn, indeP, bpre, low_eq, E in *; intros s1 s2 h Hleq; simpl.
+      cutrewrite (s1 4%Z = s2 4%Z); [| apply Hleq; simpl; eauto].
+      split; intros H x; eauto.
+    Qed.
+
+    Lemma post_lassn (tid : Fin.t ntrd) : low_assn E (bpost tid).
+    Proof.
+      unfold low_assn, Bdiv.low_assn, indeP, bpost, low_eq, E in *; intros s1 s2 h Hleq; simpl.
+      cutrewrite (s1 4%Z = s2 4%Z); [| apply Hleq; simpl; eauto].
+      split; intros H x; eauto.
+    Qed.
+
+    Notation FalseP := (fun (_ : stack) (h : pheap) => False).
+
+    Definition default : (Vector.t assn ntrd * Vector.t assn ntrd) := 
+      (init (fun _ => FalseP), init (fun _ => FalseP)).
+
+    Lemma FalseP_lassn (E' : env) : low_assn E' FalseP.
+    Proof.
+      unfold low_assn, Bdiv.low_assn, indeP; intros; tauto.
+    Qed.
+
+    Definition bspec (i : nat) :=
+      match i with
+        | 0 => (init bpre, init bpost)
+        | S _ => default
+      end.
+
+    Lemma bpre_lassn (i : nat) :
+      (forall tid : Fin.t ntrd, low_assn E (Vector.nth (fst (bspec i)) tid)) /\
+      (forall tid : Fin.t ntrd, low_assn E (Vector.nth (snd (bspec i)) tid)).
+    Proof.
+      Hint Resolve FalseP_lassn pre_lassn post_lassn.
+      split; intros tid; destruct i; simpl; rewrite init_spec; eauto.
+    Qed.
+
+    Lemma default_wf (s : stack) (h : pheap) : 
+      Aistar_v (fst default) s h <-> Aistar_v (snd default) s h.
+    Proof.
+      cutrewrite (fst default = snd default); [tauto | unfold default; eauto].
+    Qed.
+
+    Lemma barrier_wf (i : nat) (st : pstate) :
+       Aistar_v (fst (bspec i)) (fst st) (snd st) <-> Aistar_v (snd (bspec i)) (fst st) (snd st).
+    Proof.
+      destruct i; simpl; [|apply default_wf].
+      assert (
+
+  Section FoldDef.
+    Definition fold :=
+      r ::= n ;;
+      Cwhile (Bnot (r < 1%Z)) (
+        Cif (tid < (Ediv2 r)) (
+          x ::= [arr + tid + Ediv2 r] ;;
+          y ::= [arr + tid] ;;
+          [arr + tid] ::= x + y
+        ) Cskip
+      ) ;;
+      Cbarrier 0;;
+      r ::= Ediv2 r.
+  End FoldDef.
+  
+  Hypothesis n_pow2 : exists e : Z, n = two_p e.
+  
+
+
+  Definition preP :=
+    (tid 
+  Definition preP_tid (i : Fin.t ntrd) := 
+    (tid === Z_of_fin i //\\
+    (arr + Z_of_fin i) -->p (1%Qc, f (nat_of_fin i)))%assn.
+
+End Fold.
